commit remaining

txn-data-consistency/Prot_2PC_2PL.thy
@@ -29,7 +29,7 @@ record 'v global_state =
 subsubsection \<open>Events\<close>
 
 datatype 'v rm_ev = Write2 txid0 'v | Read2 txid0 'v | Prepare txid0 | RLock txid0 | WLock txid0 |
-                 NoLock txid0 | NOK txid0 | Commit txid0 | Abort txid0
+                    NoLock txid0 | NOK txid0 | Commit txid0 | Abort txid0
 datatype tm_ev = User_Commit | TM_Commit | TM_Abort | TM_ReadyC | TM_ReadyA | TM_Skip
 datatype 'v ev = RM_ev key "'v rm_ev" | TM_ev cl_id tm_ev
 
@@ -53,54 +53,48 @@ abbreviation rm_status_trans where
     \<and> rm_status (rms s' k) t = to_stat
     \<and> tm_other_rms_unchanged k s s' t"
 
-fun tid_inc :: "txid0 \<Rightarrow> txid0" where
-  "tid_inc (Tn_cl sn cl) = Tn_cl (Suc sn) cl"
+fun get_cl_txn :: "txid0 \<Rightarrow> cl_id" where
+  "get_cl_txn (Tn_cl sn cl) = cl"
 
 definition write2 where
-  "write2 s k v s' cl \<equiv> let t = (Tn_cl (tm_sn (tm s cl)) cl) in 
-                          rm_status (rms s k) t = working
+  "write2 s k v s' t \<equiv> rm_status (rms s k) t = working
                         \<and> rm_fingerpr (rms s' k) t = update_key_fp (rm_fingerpr (rms s k) t) W v
                         \<and> rm_status (rms s' k) t = working
                         \<and> rm_db (rms s' k) = rm_db (rms s k)
                         \<and> tm_other_rms_unchanged k s s' t"
 
 definition read2 where
-  "read2 s v k s' cl  \<equiv> let t = (Tn_cl (tm_sn (tm s cl)) cl) in
-                          rm_status (rms s k) t = working
+  "read2 s k v s' t  \<equiv> rm_status (rms s k) t = working
                         \<and> rm_fingerpr (rms s' k) t = update_key_fp (rm_fingerpr (rms s k) t) R v
                         \<and> rm_status (rms s' k) t = working
                         \<and> rm_db (rms s' k) = rm_db (rms s k)
                         \<and> tm_other_rms_unchanged k s s' t"
 
 definition prepare where
-  "prepare s k s' cl \<equiv> tm_status (tm s cl) = tm_prepared
-                      \<and> rm_status_trans s k s' (Tn_cl (tm_sn (tm s cl)) cl) working prepared"
+  "prepare s k s' t \<equiv> tm_status (tm s (get_cl_txn t)) = tm_prepared
+                      \<and> rm_status_trans s k s' t working prepared"
 
 definition acquire_rd_lock where \<comment>\<open>Read Lock acquired\<close>
-  "acquire_rd_lock s k s' cl \<equiv> let t = (Tn_cl (tm_sn (tm s cl)) cl) in 
-                   tm_status (tm s cl) = tm_prepared
+  "acquire_rd_lock s k s' t \<equiv> tm_status (tm s (get_cl_txn t)) = tm_prepared
                   \<and> rm_fingerpr (rms s k) t W = None
                   \<and> rm_fingerpr (rms s k) t R \<noteq> None
                   \<and> (\<forall>t'. rm_status (rms s k) t' \<in> {working, prepared, read_lock, no_lock, notokay})
                   \<and> rm_status_trans s k s' t prepared read_lock"
 
 definition acquire_wr_lock where \<comment>\<open>Write Lock acquired\<close>
-  "acquire_wr_lock s k s' cl \<equiv> let t = (Tn_cl (tm_sn (tm s cl)) cl) in 
-                   tm_status (tm s cl) = tm_prepared
+  "acquire_wr_lock s k s' t \<equiv> tm_status (tm s (get_cl_txn t)) = tm_prepared
                   \<and> rm_fingerpr (rms s k) t W \<noteq> None
                   \<and> (\<forall>t'. rm_status (rms s k) t' \<in> {working, prepared, no_lock, notokay})
                   \<and> rm_status_trans s k s' t prepared write_lock"
 
 definition acquire_no_lock where \<comment>\<open>No Lock needed\<close>
-  "acquire_no_lock s k s' cl \<equiv> let t = (Tn_cl (tm_sn (tm s cl)) cl) in 
-                   tm_status (tm s cl) = tm_prepared
-                  \<and> rm_fingerpr (rms s k) t W = None
-                  \<and> rm_fingerpr (rms s k) t R = None
-                  \<and> rm_status_trans s k s' t prepared no_lock"
+  "acquire_no_lock s k s' t \<equiv> tm_status (tm s (get_cl_txn t)) = tm_prepared
+                            \<and> rm_fingerpr (rms s k) t W = None
+                            \<and> rm_fingerpr (rms s k) t R = None
+                            \<and> rm_status_trans s k s' t prepared no_lock"
 
 definition nok where \<comment>\<open>Lock not available\<close>
-  "nok s k s' cl \<equiv> let t = (Tn_cl (tm_sn (tm s cl)) cl) in 
-                    tm_status (tm s cl) = tm_prepared \<and>
+  "nok s k s' t \<equiv> tm_status (tm s (get_cl_txn t)) = tm_prepared \<and>
                     ((rm_fingerpr (rms s k) t R \<noteq> None \<and>
                       (\<exists>t'. rm_status (rms s k) t' = write_lock)) \<or>
                      (rm_fingerpr (rms s k) t W \<noteq> None \<and>
@@ -108,9 +102,8 @@ definition nok where \<comment>\<open>Lock not available\<close>
                     rm_status_trans s k s' t prepared notokay"
 
 definition commit where
-  "commit s k s' cl \<equiv> let t = (Tn_cl (tm_sn (tm s cl)) cl) in 
-                        rm_status (rms s k) t \<in> {read_lock, write_lock, no_lock}
-                      \<and> tm_status (tm s cl) = tm_committed
+  "commit s k s' t \<equiv> rm_status (rms s k) t \<in> {read_lock, write_lock, no_lock}
+                      \<and> tm_status (tm s (get_cl_txn t)) = tm_committed
                       \<and> rm_db (rms s' k) =  update_kv t (rm_fingerpr (rms s k) t)
                                                        (tm_view (tm s)) (rm_db (rms s k)) \<comment>\<open>?\<close>
                       \<and> rm_fingerpr (rms s' k) t = Map.empty
@@ -118,9 +111,8 @@ definition commit where
                       \<and> tm_other_rms_unchanged rm s s' t"
 
 definition abort where \<comment>\<open>Locks released (aborted)\<close>
-  "abort s k s' cl \<equiv> let t = (Tn_cl (tm_sn (tm s cl)) cl) in 
-                      rm_status (rms s k) t \<in> {read_lock, write_lock, no_lock, notokay}
-                    \<and> tm_status (tm s cl) = tm_aborted
+  "abort s k s' t \<equiv> rm_status (rms s k) t \<in> {read_lock, write_lock, no_lock, notokay}
+                    \<and> tm_status (tm s (get_cl_txn t)) = tm_aborted
                     \<and> rm_db (rms s' k) = rm_db (rms s k)
                     \<and> rm_fingerpr (rms s' k) t = Map.empty
                     \<and> rm_status (rms s' k) t = aborted
@@ -150,43 +142,47 @@ definition tm_abort where
                     \<and> rms s' = rms s"
 
 definition tm_ready_c where
-  "tm_ready_c s s' \<equiv> tm_status (tm s cl) = tm_committed
-                    \<and> (\<forall>k. rm_status (rms s k) = working \<and> rm_tid (rms s k) = tid_inc (tm_tid (tm s)))
-                    \<and> tm_status (tm s' cl) = tm_init
-                    \<and> tm_sn (tm s' cl) = Suc (tm_sn (tm s cl))
-                    \<and> rms s' = rms s"
+  "tm_ready_c s s' cl \<equiv> let t = (Tn_cl (tm_sn (tm s cl)) cl) in
+                        tm_status (tm s cl) = tm_committed
+                      \<and> (\<forall>k. rm_status (rms s k) t = committed)
+                      \<and> tm_status (tm s' cl) = tm_init
+                      \<and> tm_sn (tm s' cl) = Suc (tm_sn (tm s cl))
+                      \<and> rms s' = rms s"
 
 definition tm_ready_a where
-  "tm_ready_a s s' \<equiv> tm_status (tm s cl) = tm_aborted
-                    \<and> (\<forall>k. rm_status (rms s k) = working \<and> rm_tid (rms s k) = tid_inc (tm_tid (tm s)))
-                    \<and> tm_status (tm s' cl) = tm_init
-                    \<and> tm_sn (tm s' cl) = Suc (tm_sn (tm s cl))
-                    \<and> rms s' = rms s"
+  "tm_ready_a s s' cl \<equiv> let t = (Tn_cl (tm_sn (tm s cl)) cl) in
+                        tm_status (tm s cl) = tm_aborted
+                      \<and> (\<forall>k. rm_status (rms s k) t = aborted)
+                      \<and> tm_status (tm s' cl) = tm_init
+                      \<and> tm_sn (tm s' cl) = Suc (tm_sn (tm s cl))
+                      \<and> rms s' = rms s"
 
 consts cl0 :: cl_id
 text\<open>The Event System\<close>
 definition gs_init :: "'v global_state" where
   "gs_init \<equiv> \<lparr> 
-    tm = \<lparr> tm_status = tm_init, tm_tid = Tn_cl 0 cl0, tm_view = view_init \<rparr>,
-    rms = (\<lambda>rm. \<lparr> rm_db = kvs_init, rm_fingerpr = Map.empty, 
-                  rm_status = working, rm_tid = Tn_cl 0 cl0 \<rparr>)
+    tm = (\<lambda>cl. \<lparr> tm_status = tm_init, tm_sn = 0 \<rparr>),
+    rms = (\<lambda>k. \<lparr> rm_db = [version_init],
+                 rm_fingerpr = (\<lambda>t. Map.empty), 
+                 rm_status = (\<lambda>t. working)\<rparr>)
   \<rparr>"
 
 fun gs_trans :: "'v global_state \<Rightarrow> 'v ev \<Rightarrow> 'v global_state \<Rightarrow> bool" where
-  "gs_trans s (Write2 rm k v) s' \<longleftrightarrow> write2 s rm k v s'" |
-  "gs_trans s (Read2 rm k ov) s' \<longleftrightarrow> read2 s rm k ov s'" |
-  "gs_trans s (Prepare k)    s' \<longleftrightarrow> prepare s rm s'" |
-  "gs_trans s (OK k)         s' \<longleftrightarrow> ok s rm s'" |
-  "gs_trans s (NOK k)        s' \<longleftrightarrow> nok s rm s'" |
-  "gs_trans s (Commit k)     s' \<longleftrightarrow> commit s rm s'" |
-  "gs_trans s (Abort k)      s' \<longleftrightarrow> abort s rm s'" |
-  "gs_trans s (Ready k)      s' \<longleftrightarrow> ready s rm s'" |
-  "gs_trans s User_Commit     s' \<longleftrightarrow> user_commit s s'" |
-  "gs_trans s TM_Commit       s' \<longleftrightarrow> tm_commit s s'" |
-  "gs_trans s TM_Abort        s' \<longleftrightarrow> tm_abort s s'" |
-  "gs_trans s TM_ReadyC       s' \<longleftrightarrow> tm_ready_c s s'" |
-  "gs_trans s TM_ReadyA       s' \<longleftrightarrow> tm_ready_a s s'" |
-  "gs_trans s TM_Skip         s' \<longleftrightarrow> s' = s"
+  "gs_trans s (RM_ev k (Write2 t v)) s' \<longleftrightarrow> write2 s k v s' t" |
+  "gs_trans s (RM_ev k (Read2 t v))  s' \<longleftrightarrow> read2 s k v s' t" |
+  "gs_trans s (RM_ev k (Prepare t))  s' \<longleftrightarrow> prepare s k s' t" |
+  "gs_trans s (RM_ev k (RLock t))    s' \<longleftrightarrow> acquire_rd_lock s k s' t" |
+  "gs_trans s (RM_ev k (WLock t))    s' \<longleftrightarrow> acquire_wr_lock s k s' t" |
+  "gs_trans s (RM_ev k (NoLock t))   s' \<longleftrightarrow> acquire_no_lock s k s' t" |
+  "gs_trans s (RM_ev k (NOK t))      s' \<longleftrightarrow> nok s k s' t" |
+  (*"gs_trans s (RM_ev k (Commit t))   s' \<longleftrightarrow> commit s k s'" |*)
+  "gs_trans s (RM_ev k (Abort t))    s' \<longleftrightarrow> abort s k s' t" |
+  "gs_trans s (TM_ev cl User_Commit) s' \<longleftrightarrow> user_commit s s' cl" |
+  "gs_trans s (TM_ev cl TM_Commit)   s' \<longleftrightarrow> tm_commit s s' cl" |
+  "gs_trans s (TM_ev cl TM_Abort)    s' \<longleftrightarrow> tm_abort s s' cl" |
+  "gs_trans s (TM_ev cl TM_ReadyC)   s' \<longleftrightarrow> tm_ready_c s s' cl" |
+  "gs_trans s (TM_ev cl TM_ReadyA)   s' \<longleftrightarrow> tm_ready_a s s' cl" |
+  "gs_trans s (TM_ev cl TM_Skip)     s' \<longleftrightarrow> s' = s"
 
 definition tps :: "('v ev, 'v global_state) ES" where
   "tps \<equiv> \<lparr>
@@ -194,7 +190,8 @@ definition tps :: "('v ev, 'v global_state) ES" where
     trans = gs_trans
   \<rparr>"
 
-lemmas tps_trans_defs = prepare_def ok_def nok_def commit_def abort_def ready_def
+lemmas tps_trans_defs = write2_def read2_def prepare_def acquire_rd_lock_def acquire_wr_lock_def
+                        acquire_no_lock_def nok_def (*commit_def*) abort_def
                         user_commit_def tm_commit_def tm_abort_def tm_ready_c_def tm_ready_a_def
 
 lemmas tps_defs = tps_def gs_init_def
